Constructors are capitalized

StdLib.v
@@ -15,21 +15,21 @@ Definition C (sig : Signature.t) (A : Type) : Type :=
 Module Log.
   (** Log a message on the standard output. *)
   Definition write {sig : Signature.t} (message : string) : C sig unit :=
-    C.write (Output.log (Log.Output.write message)).
+    C.Emit (Output.Log (Log.Output.Write message)).
 End Log.
 
 (** General system calls. *)
 Module System.
   (** Exit the program. *)
   Definition exit {sig : Signature.t} (_ : unit) : C sig unit :=
-    C.write (Output.system System.Output.exit).
+    C.Emit (Output.System System.Output.Exit).
 End System.
 
 (** Read a file. *)
 Module File.
   (** Read all the content of a file. *)
   Definition read {sig : Signature.t} (file_name : string) : C sig unit :=
-    C.write (Output.file (File.Output.read file_name)).
+    C.Emit (Output.File (File.Output.Read file_name)).
 End File.
 
 (** TCP client socket. *)
@@ -37,22 +37,22 @@ Module TCPClientSocket.
   (** Write a message. *)
   Definition write {sig : Signature.t} (id : TCPClientSocket.Id.t)
     (data : string) : C sig unit :=
-    C.write (Output.client_socket (TCPClientSocket.Output.write id data)).
+    C.Emit (Output.ClientSocket (TCPClientSocket.Output.Write id data)).
 
   (** Close a socket. *)
   Definition close {sig : Signature.t} (id : TCPClientSocket.Id.t)
     : C sig unit :=
-    C.write (Output.client_socket (TCPClientSocket.Output.close id)).
+    C.Emit (Output.ClientSocket (TCPClientSocket.Output.Close id)).
 End TCPClientSocket.
 
 (** TCP server socket. *)
 Module TCPServerSocket.
   (** Bind a socket. *)
   Definition bind {sig : Signature.t} (port : nat) : C sig unit :=
-    C.write (Output.server_socket (TCPServerSocket.Output.bind port)).
+    C.Emit (Output.ServerSocket (TCPServerSocket.Output.Bind port)).
 
   (** Close a socket. *)
   Definition close {sig : Signature.t} (id : TCPServerSocket.Id.t)
     : C sig unit :=
-    C.write (Output.server_socket (TCPServerSocket.Output.close id)).
+    C.Emit (Output.ServerSocket (TCPServerSocket.Output.Close id)).
 End TCPServerSocket.
