Pervasives.v
@@ -10,7 +10,7 @@ Open Local Scope string.
 Module Log.
   Module Output.
     Inductive t : Set :=
-    | write (message : string).
+    | Write (message : string).
   End Output.
 End Log.
 
@@ -19,14 +19,14 @@ Module File.
   (** Incoming events. *)
   Module Input.
     Inductive t : Set :=
-    | read (file_name : string) (content : string)
+    | Read (file_name : string) (content : string)
       (** All the file content had been read. *).
   End Input.
 
   (** Generated events. *)
   Module Output.
     Inductive t : Set :=
-    | read (file_name : string) (** Read all the content of a file. *).
+    | Read (file_name : string) (** Read all the content of a file. *).
   End Output.
 End File.
 
@@ -34,7 +34,7 @@ End File.
 Module System.
   Module Output.
     Inductive t : Set :=
-    | exit.
+    | Exit.
   End Output.
 End System.
 
@@ -46,27 +46,27 @@ Module TCPClientSocket.
 
     (** An integer. *)
     Inductive t : Set :=
-    | new : nat -> t.
+    | New : nat -> t.
 
     (** Test equality. *)
     Definition eqb (id1 id2 : t) : bool :=
       match (id1, id2) with
-      | (new id1, new id2) => Nat.eqb id1 id2
+      | (New id1, New id2) => Nat.eqb id1 id2
       end.
   End Id.
 
   (** Incoming events. *)
   Module Input.
     Inductive t : Set :=
-    | accepted (id : Id.t)
-    | read (id : Id.t) (content : string).
+    | Accepted (id : Id.t)
+    | Read (id : Id.t) (content : string).
   End Input.
 
   (** Generated events. *)
   Module Output.
     Inductive t : Set :=
-    | write (id : Id.t) (message : string)
-    | close (id : Id.t).
+    | Write (id : Id.t) (message : string)
+    | Close (id : Id.t).
   End Output.
 End TCPClientSocket.
 
@@ -76,37 +76,37 @@ Module TCPServerSocket.
   Module Id.
     (** An integer. *)
     Inductive t : Set :=
-    | new : nat -> t.
+    | New : nat -> t.
   End Id.
 
   (** Incoming events. *)
   Module Input.
     Inductive t : Set :=
-    | bound (id : Id.t).
+    | Bound (id : Id.t).
   End Input.
 
   (** Generated events. *)
   Module Output.
     Inductive t : Set :=
-    | bind (port : nat)
-    | close (id : Id.t).
+    | Bind (port : nat)
+    | Close (id : Id.t).
   End Output.
 End TCPServerSocket.
 
 (** Incoming events. *)
 Module Input.
   Inductive t : Set :=
-  | file : File.Input.t -> t
-  | client_socket : TCPClientSocket.Input.t -> t
-  | server_socket : TCPServerSocket.Input.t -> t.
+  | File : File.Input.t -> t
+  | ClientSocket : TCPClientSocket.Input.t -> t
+  | ServerSocket : TCPServerSocket.Input.t -> t.
 End Input.
 
 (** Generated events. *)
 Module Output.
   Inductive t : Set :=
-  | log : Log.Output.t -> t
-  | file : File.Output.t -> t
-  | system : System.Output.t -> t
-  | client_socket : TCPClientSocket.Output.t -> t
-  | server_socket : TCPServerSocket.Output.t -> t.
+  | Log : Log.Output.t -> t
+  | File : File.Output.t -> t
+  | System : System.Output.t -> t
+  | ClientSocket : TCPClientSocket.Output.t -> t
+  | ServerSocket : TCPServerSocket.Output.t -> t.
 End Output.
